todo.md
@@ -3,9 +3,15 @@
 # Todo #
 
     * tactic for monotonicity in predicate calculus
-    * ~reduce soundness of leads-to properties to assumptions about transient~
-	* ~prove soundness of unitb.models.sched~
+    * ~~reduce soundness of leads-to properties to assumptions about transient~~
+	* ~~prove soundness of unitb.models.sched~~
 	* prove that unitb.models.sched are inhabited
-	* in unitb.models.sched, give a rule that relies only on predicate
-      calculus and UNITY logic
-	* study model where the state space is encoded in the
+	* ~~in unitb.models.sched, give a rule that relies only on predicate
+      calculus and UNITY logic~~
+	* study model where the invariant is encoded in the state space
+	* refinement
+	  * schedules
+	  * simulation
+	  * splitting / merging
+	  * data refinement
+	* shared variable decomposition
